Remove Comparison.dfy and revert to plain relations, general cleanup

src/Relations/Relations.dfy
@@ -1,46 +1,72 @@
+// RUN: %dafny /compile:0 "%s"
+
+/*******************************************************************************
+*  Copyright by the contributors to the Dafny Project
+*  SPDX-License-Identifier: MIT 
+*******************************************************************************/
+
 module Relations { 
 
-    predicate Reflexive<T(!new)>(R: (T, T) -> bool) 
-    {
-        forall x :: R(x, x)
-    }
+  predicate Reflexive<T(!new)>(R: (T, T) -> bool) {
+    forall x :: R(x, x)
+  }
 
-    predicate AntiSymmetric<T(!new)>(R: (T, T) -> bool) 
-    {
-        forall x, y :: R(x, y) && R(y, x) ==> x == y
-    }
+  predicate Irreflexive<T(!new)>(R: (T, T) -> bool) {
+    forall x :: !R(x, x)
+  }
 
-    predicate Connected<T(!new)>(R: (T, T) -> bool) 
-    {
-        forall x, y :: R(x, y) || R(y, x)
-    }
+  predicate AntiSymmetric<T(!new)>(R: (T, T) -> bool) {
+    forall x, y :: R(x, y) && R(y, x) ==> x == y
+  }
 
-    predicate TotalOrdering<T(!new)>(R: (T, T) -> bool) 
-    {
+  predicate Connected<T(!new)>(R: (T, T) -> bool) {
+    forall x, y :: x != y ==> R(x, y) || R(y, x)
+  }
+
+  predicate StronglyConnected<T(!new)>(R: (T, T) -> bool) {
+    forall x, y :: R(x, y) || R(y, x)
+  }
+
+  predicate Transitive<T(!new)>(R: (T, T) -> bool) {
+    forall x, y, z :: R(x, y) && R(y, z) ==> R(x, z)
+  }
+
+  predicate TotalOrdering<T(!new)>(R: (T, T) -> bool) {
     && Reflexive(R)
     && AntiSymmetric(R)
     && Transitive(R)
+    && StronglyConnected(R)
+  }  
+
+  predicate StrictTotalOrdering<T(!new)>(R: (T, T) -> bool) {
+    && Irreflexive(R)
+    && AntiSymmetric(R)
+    && Transitive(R)
     && Connected(R)
-    }  
+  }  
 
-    /*
-    * To be _trichotomous_ means that for any two `x` and `y`,
-    * EXACTLY one of the following three conditions holds:
-    *   - less(x, y)
-    *   - x == y
-    *   - less(y, x)
-    * Note that being trichotomous implies being irreflexive.
-    */
+  predicate method SortedBy<T>(a: seq<T>, less: (T, T) -> bool) {
+    forall i, j | 0 <= i < j < |a| :: less(a[i], a[j])
+  }
 
-    predicate Trichotomous<T(!new)>(less: (T, T) -> bool) 
-    {
-        (forall x, y :: less(x, y) || x == y || less(y, x)) &&  // at least one of the three
-        (forall x, y :: less(x, y) && less(y, x) ==> false) &&  // not both of the less's
-        (forall x, y :: less(x, y) ==> x != y)  // not a less and the equality
-    }
+  lemma LemmaNewFirstElementStillSortedBy<T>(x: T, s: seq<T>, less: (T, T) -> bool) 
+    requires SortedBy(s, less)
+    requires |s| == 0 || less(x, s[0])
+    requires TotalOrdering(less)
+    ensures SortedBy([x] + s, less)
+  {}  
 
-    predicate Transitive<T(!new)>(R: (T, T) -> bool) 
-    {
-        forall x, y, z :: R(x, y) && R(y, z) ==> R(x, z)
-    }
+  /*
+  * To be _trichotomous_ means that for any two `x` and `y`,
+  * EXACTLY one of the following three conditions holds:
+  *   - less(x, y)
+  *   - x == y
+  *   - less(y, x)
+  * Note that being trichotomous implies being irreflexive.
+  */
+  predicate Trichotomous<T(!new)>(less: (T, T) -> bool) {
+    (forall x, y :: less(x, y) || x == y || less(y, x)) &&  // at least one of the three
+    (forall x, y :: less(x, y) && less(y, x) ==> false) &&  // not both of the less's
+    (forall x, y :: less(x, y) ==> x != y)  // not a less and the equality
+  }
 }
