src/Collections/Sequences/MergeSort.dfy
@@ -1,16 +1,21 @@
-include "../../Relations/Comparison.dfy"
+// RUN: %dafny /compile:0 "%s"
 
-module Seq.MergeSort{
+/*******************************************************************************
+*  Copyright by the contributors to the Dafny Project
+*  SPDX-License-Identifier: MIT 
+*******************************************************************************/
 
-  import opened Relations.Comparison
+include "../../Relations/Relations.dfy"
+
+module Seq.MergeSort {
+
+  import opened Relations
 
   //Splits a sequence in two, sorts the two subsequences using itself, and merge the two sorted sequences using `MergeSortedWith`
-  function method MergeSortBy<T>(a: seq<T>, compare: (T, T) -> CompResult): (result :seq<T>)
-    requires Total?(compare)
-    requires Connected(compare)
+  function method MergeSortBy<T>(a: seq<T>, compare: (T, T) -> bool): (result :seq<T>)
+    requires TotalOrdering(compare)
     ensures multiset(a) == multiset(result)
-    ensures SortedBy(result,compare)
-
+    ensures SortedBy(result, compare)
   {
     if |a| <= 1 then
       a
@@ -22,32 +27,30 @@ module Seq.MergeSort{
 
       var leftSorted := MergeSortBy(left, compare);
       var rightSorted := MergeSortBy(right, compare);
-      
+
       MergeSortedWith(leftSorted, rightSorted, compare)
   }
 
-  function method {:tailrecursion} MergeSortedWith<T>(left: seq<T>, right: seq<T>,  compare: (T, T) -> CompResult) : (result :seq<T>)
-    requires SortedBy(left,compare)
-    requires SortedBy(right,compare)
-    requires Comparison.Total?(compare)
-    requires Connected(compare)
+  function method {:tailrecursion} MergeSortedWith<T>(left: seq<T>, right: seq<T>, compare: (T, T) -> bool) : (result :seq<T>)
+    requires SortedBy(left, compare)
+    requires SortedBy(right, compare)
+    requires TotalOrdering(compare)
     ensures multiset(left + right) == multiset(result)
-    ensures SortedBy(result,compare)
+    ensures SortedBy(result, compare)
   {
     if |left| == 0 then
       right
     else if |right| == 0 then
       left
-    else if compare(left[0],right[0]).LessThan? then
+    else if compare(left[0], right[0]) then
       LemmaNewFirstElementStillSortedBy(left[0], MergeSortedWith(left[1..], right, compare), compare);
       assert left == [left[0]] + left[1..];
 
-      [left[0]] +  MergeSortedWith(left[1..], right, compare)
-      
+      [left[0]] + MergeSortedWith(left[1..], right, compare)
 
-      else
-        LemmaNewFirstElementStillSortedBy(right[0], MergeSortedWith(left, right[1..], compare), compare);
-        assert right == [right[0]] + right[1..];
+    else
+      LemmaNewFirstElementStillSortedBy(right[0], MergeSortedWith(left, right[1..], compare), compare);
+      assert right == [right[0]] + right[1..];
 
       [right[0]] + MergeSortedWith(left, right[1..], compare)
   }
